Added `implies not`

src/Operational.thy
@@ -57,6 +57,14 @@ inductive operational_semantics_elim :: "config \<Rightarrow> config \<Rightarro
   "(* consistent_run ((K\<^sub>1 \<Up> n) # (K\<^sub>2 \<Up> n) # \<Gamma>) \<Longrightarrow> *)
    \<Gamma>, n \<turnstile> (K\<^sub>1 implies K\<^sub>2) # \<Psi> \<triangleright> \<Phi>
      \<hookrightarrow>\<^sub>e  K\<^sub>1 \<Up> n # K\<^sub>2 \<Up> n # \<Gamma>, n \<turnstile> \<Psi> \<triangleright> (K\<^sub>1 implies K\<^sub>2) # \<Phi>"
+| implies_not_e1:
+  "(* consistent_run (K\<^sub>1 \<not>\<Up> n # \<Gamma>) \<Longrightarrow> *)
+   \<Gamma>, n \<turnstile> (K\<^sub>1 implies not K\<^sub>2) # \<Psi> \<triangleright> \<Phi>
+     \<hookrightarrow>\<^sub>e  K\<^sub>1 \<not>\<Up> n # \<Gamma>, n \<turnstile> \<Psi> \<triangleright> (K\<^sub>1 implies not K\<^sub>2) # \<Phi>"
+| implies_not_e2:
+  "(* consistent_run ((K\<^sub>1 \<Up> n) # (K\<^sub>2 \<Up> n) # \<Gamma>) \<Longrightarrow> *)
+   \<Gamma>, n \<turnstile> (K\<^sub>1 implies not K\<^sub>2) # \<Psi> \<triangleright> \<Phi>
+     \<hookrightarrow>\<^sub>e  K\<^sub>1 \<Up> n # K\<^sub>2 \<not>\<Up> n # \<Gamma>, n \<turnstile> \<Psi> \<triangleright> (K\<^sub>1 implies not K\<^sub>2) # \<Phi>"
 | iff_e1:
   "\<Gamma>, n \<turnstile> (K\<^sub>1 iff K\<^sub>2) # \<Psi> \<triangleright> \<Phi>
      \<hookrightarrow>\<^sub>e  K\<^sub>1 \<not>\<Up> n # K\<^sub>2 \<not>\<Up> n # \<Gamma>, n \<turnstile> \<Psi> \<triangleright> (K\<^sub>1 iff K\<^sub>2) # \<Phi>"
@@ -162,6 +170,12 @@ lemma Cnext_solve_implies:
           \<supseteq> { K\<^sub>1 \<not>\<Up> n # \<Gamma>, n \<turnstile> \<Psi> \<triangleright> (K\<^sub>1 implies K\<^sub>2) # \<Phi>,
               K\<^sub>1 \<Up> n # K\<^sub>2 \<Up> n # \<Gamma>, n \<turnstile> \<Psi> \<triangleright> (K\<^sub>1 implies K\<^sub>2) # \<Phi>}"
   by (simp add: operational_semantics_step.simps operational_semantics_elim.implies_e1 operational_semantics_elim.implies_e2)
+
+lemma Cnext_solve_implies_not:
+  shows "\<C>\<^sub>n\<^sub>e\<^sub>x\<^sub>t (\<Gamma>, n \<turnstile> (K\<^sub>1 implies not K\<^sub>2) # \<Psi> \<triangleright> \<Phi>)
+          \<supseteq> { (K\<^sub>1 \<not>\<Up> n) # \<Gamma>, n \<turnstile> \<Psi> \<triangleright> (K\<^sub>1 implies not K\<^sub>2) # \<Phi>,
+              (K\<^sub>1 \<Up> n) # (K\<^sub>2 \<not>\<Up> n) # \<Gamma>, n \<turnstile> \<Psi> \<triangleright> (K\<^sub>1 implies not K\<^sub>2) # \<Phi>}"
+  by (simp add: operational_semantics_step.simps operational_semantics_elim.implies_not_e1 operational_semantics_elim.implies_not_e2)
 
 lemma Cnext_solve_iff:
   shows "\<C>\<^sub>n\<^sub>e\<^sub>x\<^sub>t (\<Gamma>, n \<turnstile> (K\<^sub>1 iff K\<^sub>2) # \<Psi> \<triangleright> \<Phi>)
