src/Coinductive_Prop.thy
@@ -27,6 +27,8 @@ fun TESL_interpretation_atomic_stepwise
         { \<rho>. \<forall>n\<ge>i. R (time ((Rep_run \<rho>) n K\<^sub>1), time ((Rep_run \<rho>) n K\<^sub>2)) }"
   | "\<lbrakk> master implies slave \<rbrakk>\<^sub>T\<^sub>E\<^sub>S\<^sub>L\<^bsup>\<ge> i\<^esup> =
         { \<rho>. \<forall>n\<ge>i. hamlet ((Rep_run \<rho>) n master) \<longrightarrow> hamlet ((Rep_run \<rho>) n slave) }"
+  | "\<lbrakk> master implies not slave \<rbrakk>\<^sub>T\<^sub>E\<^sub>S\<^sub>L\<^bsup>\<ge> i\<^esup> =
+        { \<rho>. \<forall>n\<ge>i. hamlet ((Rep_run \<rho>) n master) \<longrightarrow> \<not> hamlet ((Rep_run \<rho>) n slave) }"
   | "\<lbrakk> K\<^sub>1 iff K\<^sub>2 \<rbrakk>\<^sub>T\<^sub>E\<^sub>S\<^sub>L\<^bsup>\<ge> i\<^esup> =
         { \<rho>. \<forall>n\<ge>i. hamlet ((Rep_run \<rho>) n K\<^sub>1) \<longleftrightarrow> hamlet ((Rep_run \<rho>) n K\<^sub>2) }"
   | "\<lbrakk> master anytime implies slave \<rbrakk>\<^sub>T\<^sub>E\<^sub>S\<^sub>L\<^bsup>\<ge> i\<^esup> =
@@ -79,6 +81,10 @@ lemma TESL_interp_unfold_stepwise_implies:
   shows "\<lbrakk> master implies slave \<rbrakk>\<^sub>T\<^sub>E\<^sub>S\<^sub>L = \<Inter> {Y. \<exists>n::nat. Y = \<lbrakk> master implies slave \<rbrakk>\<^sub>T\<^sub>E\<^sub>S\<^sub>L\<^bsup>\<ge> n\<^esup>}"
   by auto
 
+lemma TESL_interp_unfold_stepwise_implies_not:
+  shows "\<lbrakk> master implies not slave \<rbrakk>\<^sub>T\<^sub>E\<^sub>S\<^sub>L = \<Inter> {Y. \<exists>n::nat. Y = \<lbrakk> master implies not slave \<rbrakk>\<^sub>T\<^sub>E\<^sub>S\<^sub>L\<^bsup>\<ge> n\<^esup>}"
+  by auto
+
 lemma TESL_interp_unfold_stepwise_iff:
   shows "\<lbrakk> master iff slave \<rbrakk>\<^sub>T\<^sub>E\<^sub>S\<^sub>L = \<Inter> {Y. \<exists>n::nat. Y = \<lbrakk> master iff slave \<rbrakk>\<^sub>T\<^sub>E\<^sub>S\<^sub>L\<^bsup>\<ge> n\<^esup>}"
   by auto
@@ -113,7 +119,7 @@ theorem TESL_interp_unfold_stepwise_positive_atoms:
 theorem TESL_interp_unfold_stepwise_negative_atoms:
   assumes "\<not> positive_atom \<phi>"
   shows "\<lbrakk> \<phi> \<rbrakk>\<^sub>T\<^sub>E\<^sub>S\<^sub>L = \<Inter> {Y. \<exists>n::nat. Y = \<lbrakk> \<phi> \<rbrakk>\<^sub>T\<^sub>E\<^sub>S\<^sub>L\<^bsup>\<ge> n\<^esup>}"
-  by (smt Collect_cong TESL_interp_unfold_stepwise_not TESL_interp_unfold_stepwise_implies
+  by (smt Collect_cong TESL_interp_unfold_stepwise_not TESL_interp_unfold_stepwise_implies TESL_interp_unfold_stepwise_implies_not
       TESL_interp_unfold_stepwise_tagrel TESL_interp_unfold_stepwise_tagrelgen TESL_interp_unfold_stepwise_iff
       TESL_interp_unfold_stepwise_implies_anytime TESL_interp_unfold_stepwise_timedelayed assms
       positive_atom.elims(3))
@@ -242,6 +248,18 @@ lemma TESL_interp_stepwise_implies_coind_unfold:
     then show ?thesis by auto
   qed
 
+lemma TESL_interp_stepwise_implies_not_coind_unfold:
+  shows "\<lbrakk> master implies not slave \<rbrakk>\<^sub>T\<^sub>E\<^sub>S\<^sub>L\<^bsup>\<ge> n\<^esup> =
+    (\<lbrakk> master \<not>\<Up> n \<rbrakk>\<^sub>s\<^sub>y\<^sub>m\<^sub>r\<^sub>u\<^sub>n \<union> \<lbrakk> master \<Up> n \<rbrakk>\<^sub>s\<^sub>y\<^sub>m\<^sub>r\<^sub>u\<^sub>n \<inter> \<lbrakk> slave \<not>\<Up> n \<rbrakk>\<^sub>s\<^sub>y\<^sub>m\<^sub>r\<^sub>u\<^sub>n)
+    \<inter> \<lbrakk> master implies not slave \<rbrakk>\<^sub>T\<^sub>E\<^sub>S\<^sub>L\<^bsup>\<ge> Suc n\<^esup>"
+  proof -
+    have "{ \<rho>. \<forall>m\<ge>n. hamlet ((Rep_run \<rho>) m master) \<longrightarrow> \<not> hamlet ((Rep_run \<rho>) m slave) }
+          = { \<rho>. hamlet ((Rep_run \<rho>) n master) \<longrightarrow> \<not> hamlet ((Rep_run \<rho>) n slave) }
+          \<inter> { \<rho>. \<forall>m\<ge>Suc n. hamlet ((Rep_run \<rho>) m master) \<longrightarrow> \<not> hamlet ((Rep_run \<rho>) m slave) }"
+      by (smt Collect_cong Collect_conj_eq Suc_leD eq_refl le_antisym not_less_eq_eq)
+    then show ?thesis by auto
+  qed
+
 lemma TESL_interp_stepwise_iff_coind_unfold:
   shows "\<lbrakk> K\<^sub>1 iff K\<^sub>2 \<rbrakk>\<^sub>T\<^sub>E\<^sub>S\<^sub>L\<^bsup>\<ge> n\<^esup> =
     (\<lbrakk> K\<^sub>1 \<not>\<Up> n \<rbrakk>\<^sub>s\<^sub>y\<^sub>m\<^sub>r\<^sub>u\<^sub>n \<inter> \<lbrakk> K\<^sub>2 \<not>\<Up> n \<rbrakk>\<^sub>s\<^sub>y\<^sub>m\<^sub>r\<^sub>u\<^sub>n \<union> \<lbrakk> K\<^sub>1 \<Up> n \<rbrakk>\<^sub>s\<^sub>y\<^sub>m\<^sub>r\<^sub>u\<^sub>n \<inter> \<lbrakk> K\<^sub>2 \<Up> n \<rbrakk>\<^sub>s\<^sub>y\<^sub>m\<^sub>r\<^sub>u\<^sub>n)
@@ -258,7 +276,13 @@ lemma TESL_interp_stepwise_implies_anytime_coind_unfold:
   shows "\<lbrakk> master anytime implies slave \<rbrakk>\<^sub>T\<^sub>E\<^sub>S\<^sub>L\<^bsup>\<ge> n\<^esup> =
     (\<lbrakk> master \<not>\<Up> n \<rbrakk>\<^sub>s\<^sub>y\<^sub>m\<^sub>r\<^sub>u\<^sub>n \<union> \<lbrakk> master \<Up> n \<rbrakk>\<^sub>s\<^sub>y\<^sub>m\<^sub>r\<^sub>u\<^sub>n \<inter> \<lbrakk> slave sporadic anytime \<rbrakk>\<^sub>T\<^sub>E\<^sub>S\<^sub>L\<^bsup>\<ge> n\<^esup>)
     \<inter> \<lbrakk> master anytime implies slave \<rbrakk>\<^sub>T\<^sub>E\<^sub>S\<^sub>L\<^bsup>\<ge> Suc n\<^esup>"
-  sorry
+  proof -
+    have "{ \<rho>. \<forall>m\<ge>n. hamlet ((Rep_run \<rho>) m master) \<longrightarrow> (\<exists>p \<ge> m. hamlet ((Rep_run \<rho>) p slave)) }
+         = { \<rho>. hamlet ((Rep_run \<rho>) n master) \<longrightarrow> (\<exists>p \<ge> n. hamlet ((Rep_run \<rho>) p slave)) }
+         \<inter> { \<rho>. \<forall>m\<ge>Suc n. hamlet ((Rep_run \<rho>) m master) \<longrightarrow> (\<exists>p \<ge> m. hamlet ((Rep_run \<rho>) p slave)) }"
+      by (smt Collect_cong Collect_conj_eq Suc_leD eq_refl le_antisym not_less_eq_eq)
+    then show ?thesis by auto
+  qed
 
 lemma TESL_interp_stepwise_timedelayed_coind_unfold:
   shows "\<lbrakk> master time-delayed by \<delta>\<tau> on measuring implies slave \<rbrakk>\<^sub>T\<^sub>E\<^sub>S\<^sub>L\<^bsup>\<ge> n\<^esup> =
@@ -329,6 +353,9 @@ lemma TESL_interpretation_stepwise_zero:
     then show ?case by simp
   next
     case (Implies x1 x2)
+    then show ?case by simp
+  next
+    case (ImpliesNot x1 x2)
     then show ?case by simp
   next
     case (Iff x1 x2)
@@ -526,6 +553,13 @@ lemma HeronConf_interp_stepwise_implies_cases:
         by (simp add: Int_Un_distrib2 inf_sup_aci(2))
     qed
   qed
+
+lemma HeronConf_interp_stepwise_implies_not_cases:
+  shows "\<lbrakk> \<Gamma>, n \<turnstile> (K\<^sub>1 implies not K\<^sub>2) # \<Psi> \<triangleright> \<Phi> \<rbrakk>\<^sub>c\<^sub>o\<^sub>n\<^sub>f\<^sub>i\<^sub>g
+          = \<lbrakk> (K\<^sub>1 \<not>\<Up> n) # \<Gamma>, n \<turnstile> \<Psi> \<triangleright> (K\<^sub>1 implies not K\<^sub>2) # \<Phi> \<rbrakk>\<^sub>c\<^sub>o\<^sub>n\<^sub>f\<^sub>i\<^sub>g
+          \<union> \<lbrakk> (K\<^sub>1 \<Up> n) # (K\<^sub>2 \<not>\<Up> n) # \<Gamma>, n \<turnstile> \<Psi> \<triangleright> (K\<^sub>1 implies not K\<^sub>2) # \<Phi> \<rbrakk>\<^sub>c\<^sub>o\<^sub>n\<^sub>f\<^sub>i\<^sub>g"
+  by (smt HeronConf_interpretation.simps Int_commute Int_left_commute TESL_interp_stepwise_implies_not_coind_unfold
+      TESL_interpretation_stepwise_cons_morph inf_sup_distrib2 symbolic_run_interp_cons_morph)
 
 lemma HeronConf_interp_stepwise_iff_cases:
   shows "\<lbrakk> \<Gamma>, n \<turnstile> (K\<^sub>1 iff K\<^sub>2) # \<Psi> \<triangleright> \<Phi> \<rbrakk>\<^sub>c\<^sub>o\<^sub>n\<^sub>f\<^sub>i\<^sub>g
