src/Denotational.thy
@@ -27,6 +27,8 @@ fun TESL_interpretation_atomic
         { \<rho>. \<forall>n::nat. R (time ((Rep_run \<rho>) n K\<^sub>1), time ((Rep_run \<rho>) n K\<^sub>2)) }"
   | "\<lbrakk> master implies slave \<rbrakk>\<^sub>T\<^sub>E\<^sub>S\<^sub>L =
         { \<rho>. \<forall>n::nat. hamlet ((Rep_run \<rho>) n master) \<longrightarrow> hamlet ((Rep_run \<rho>) n slave) }"
+  | "\<lbrakk> master implies not slave \<rbrakk>\<^sub>T\<^sub>E\<^sub>S\<^sub>L =
+        { \<rho>. \<forall>n::nat. hamlet ((Rep_run \<rho>) n master) \<longrightarrow> \<not> hamlet ((Rep_run \<rho>) n slave) }"
   | "\<lbrakk> K\<^sub>1 iff K\<^sub>2 \<rbrakk>\<^sub>T\<^sub>E\<^sub>S\<^sub>L =
         { \<rho>. \<forall>n::nat. hamlet ((Rep_run \<rho>) n K\<^sub>1) \<longleftrightarrow> hamlet ((Rep_run \<rho>) n K\<^sub>2) }"
   | "\<lbrakk> master anytime implies slave \<rbrakk>\<^sub>T\<^sub>E\<^sub>S\<^sub>L =
